theories/FOL/FOL_undec.v
@@ -11,14 +11,35 @@ Qed.
 Lemma undecidable_FOLstar_valid : undecidable FOL*_valid.
 Proof.
    apply (undecidability_from_reducibility PCPb_undec).
+   apply PCPb_to_FOL.valid_star_red.
+Qed.
+
+Lemma undecidable_FOL_valid : undecidable FOL_valid.
+Proof.
+   apply (undecidability_from_reducibility PCPb_undec).
    apply PCPb_to_FOL.valid_red.
 Qed.
 
-(* Lemma undecidable_FOL_satis : undecidable FOL_satis.
+(*Lemma undecidable_comp X (P : X -> Prop) :
+  undecidable (compl P) -> undecidable P.
 Proof.
-   apply (undecidability_from_reducibility PCPb_undec).
-   apply PCPb_to_FOL.satis_red.
-Qed. *)
+  intros H H'. apply H. rewrite DecidabilityFacts.decidable_iff in *.
+  destruct H' as [d]. split. intros x. destruct (d x).
+  - right. intros Hx. now apply Hx.
+  - now left.
+Qed.
+
+Lemma reducible_comp X Y (P : X -> Prop) (Q : Y -> Prop) :
+  P ⪯ Q -> compl P ⪯ compl Q.
+Proof.
+  intros [f Hf]. exists f. firstorder.
+Qed.*)
+
+(*Lemma undecidable_FOL_satis : undecidable FOL_satis.
+Proof.
+  apply (undecidability_from_reducibility PCPb_undec).
+  
+Qed.*)
 
 Lemma undecidable_FOL_valid_intu : undecidable FOL_valid_intu.
 Proof.
